proofs/core/IndPropLemmas.v
@@ -1,0 +1,388 @@
+(*Typing and well-formedness results for indprops*)
+Require Export Typing.
+Require Export Interp.
+
+Section Lemmas.
+
+Context {gamma: context} (gamma_valid: valid_context gamma).
+
+Lemma in_indpred_valid_aux {l: list (predsym * list formula)}
+(l_in: In l (indpreds_of_context gamma)):
+Forall (fun y => let p := fst y in
+  let fs := snd y in 
+  (Forall (fun x =>
+  formula_typed gamma x /\
+  closed_formula x /\
+  valid_ind_form p x /\
+  asubset (fmla_type_vars x) (list_to_aset (s_params p))
+  )) fs) l.
+Proof.
+  apply valid_context_defs in gamma_valid.
+  rewrite Forall_forall in gamma_valid.
+  rename gamma_valid into Hval.
+  pose proof (in_indpreds_of_context gamma l l_in) as Hinl.
+  destruct Hinl as [l2 [Hinl2 Hl]]; subst.
+  specialize (Hval _ Hinl2).
+  simpl in Hval.
+  unfold indprop_valid in Hval. simpl.
+  destruct Hval.
+  unfold indprop_valid_type in H.
+  clear -H. induction l2; simpl in *; auto.
+  inversion H; subst.
+  destruct a. simpl in *. apply Forall_cons; auto.
+Qed.
+
+Lemma in_indpred_valid {l: list (predsym * list formula)}
+  (l_in: In l (indpreds_of_context gamma)):
+  Forall (Forall (formula_typed gamma)) (map snd l).
+Proof.
+  pose proof (in_indpred_valid_aux l_in).
+  clear -H.
+  induction l; simpl in *; auto.
+  inversion H; subst.
+  constructor; auto. revert H2. apply Forall_impl.
+  intros. apply H0.
+Qed.
+
+Lemma in_indpred_valid_ind_form {l: list (predsym * list formula)}
+(l_in: In l (indpreds_of_context gamma)):
+Forall (fun t => Forall (valid_ind_form (fst t)) (snd t)) l.
+Proof.
+  pose proof (in_indpred_valid_aux l_in).
+  revert H. apply Forall_impl; simpl; intros t.
+  apply Forall_impl; intros. apply H.
+Qed. 
+
+Lemma in_indpred_positive {l: list (predsym * list formula)}
+(l_in: In l (indpreds_of_context gamma)):
+Forall (Forall (ind_positive (map fst l))) (map snd l).
+Proof.
+  (*Need to prove directly - not in previous*)
+  apply valid_context_defs in gamma_valid.
+  rewrite Forall_forall in gamma_valid.
+  rename gamma_valid into Hval.
+  pose proof (in_indpreds_of_context gamma l l_in) as Hinl.
+  destruct Hinl as [l2 [Hinl2 Hl]]; subst.
+  specialize (Hval _ Hinl2).
+  simpl in Hval.
+  unfold indprop_valid in Hval.
+  destruct Hval as [_ [Hpos _]].
+  unfold indpred_positive in Hpos.
+  assert ((map fst (get_indpred l2)) =
+  (map (fun i : indpred_def => match i with
+                                         | ind_def p _ => p
+                                         end) l2)). {
+    clear. induction l2; simpl; auto. rewrite IHl2. f_equal.
+    destruct a; reflexivity.
+  }
+  rewrite <- H in Hpos.
+  assert ((map snd (get_indpred l2) = (map (fun i : indpred_def => match i with
+  | ind_def _ fs => map snd fs
+  end) l2))). {
+    clear. induction l2; simpl; auto.
+    rewrite IHl2. f_equal. destruct a; reflexivity.
+  }
+  rewrite <- H0 in Hpos.
+  clear H H0.
+  rewrite <- Forall_concat. apply Hpos.
+Qed.
+
+Lemma in_indpred_closed {l: list (predsym * list formula)}
+(l_in: In l (indpreds_of_context gamma)):
+Forall (Forall (fun f0 : formula => closed_formula f0)) (map snd l).
+Proof.
+  pose proof (in_indpred_valid_aux l_in).
+  rewrite Forall_map.
+  revert H; simpl; apply Forall_impl; intros a.
+  apply Forall_impl; intros; apply H.
+Qed.
+
+Lemma in_indpred_params {l: list (predsym * list formula)}
+(l_in: In l (indpreds_of_context gamma)):
+Forall_eq (fun x : predsym => s_params x) (map fst l).
+Proof.
+  apply valid_context_defs in gamma_valid.
+  rewrite Forall_forall in gamma_valid.
+  rename gamma_valid into Hval.
+  pose proof (in_indpreds_of_context gamma l l_in) as Hinl.
+  destruct Hinl as [l2 [Hinl2 Hl]]; subst.
+  specialize (Hval _ Hinl2).
+  simpl in Hval.
+  destruct Hval as [_ [_ [Hunif _]]].
+  unfold indpred_params_same in Hunif.
+  revert Hunif.
+  rewrite !Forall_eq_iff; auto.
+  intros. rewrite in_map_iff in H, H0.
+  destruct H as [[p1 fs1] [Hp1 Hinp1]];
+  destruct H0 as [[p2 fs2] [Hp2 Hinp2]];
+  simpl in *; subst.
+  unfold get_indpred in Hinp1, Hinp2.
+  rewrite in_map_iff in Hinp1, Hinp2.
+  destruct Hinp1 as [d1 [Hd1 Hind1]];
+  destruct Hinp2 as [d2 [Hd2 Hind2]].
+  specialize (Hunif _ _ Hind1 Hind2).
+  destruct d1; destruct d2; simpl in *.
+  inversion Hd1; inversion Hd2; subst; auto.
+Qed.
+
+Lemma in_indpred_typevars {l: list (predsym * list formula)} {p: predsym}
+(l_in: In l (indpreds_of_context gamma))
+(p_in: pred_in_indpred p l):
+Forall (fun f : formula => asubset (fmla_type_vars f) (list_to_aset (s_params p)))
+  (concat (map snd l)).
+Proof.
+  pose proof (in_indpred_valid_aux l_in).
+  rewrite Forall_concat.
+  rewrite Forall_map.
+  revert H; simpl; rewrite !Forall_forall; intros.
+  specialize (H _ H0).
+  revert H.
+  rewrite !Forall_forall; intros.
+  specialize (H _ H1).
+  assert (s_params (fst x) = s_params p). {
+    pose proof (in_indpred_params l_in).
+    rewrite Forall_eq_iff in H2.
+    specialize (H2 (fst x) p).
+    apply H2.
+    rewrite in_map_iff. exists x. auto.
+    apply in_bool_In in p_in. auto.
+  }
+  rewrite <- H2. apply H.
+Qed.
+
+Lemma in_indpred_unif  {l: list (predsym * list formula)} {p: predsym}
+(l_in: In l (indpreds_of_context gamma))
+(p_in: pred_in_indpred p l):
+Forall (fun f => pred_with_params_fmla (map fst l) (s_params p) f) 
+  (concat (map snd l)).
+Proof.
+  pose proof (in_indpred_params l_in) as Halleq.
+  apply valid_context_defs in gamma_valid.
+  rewrite Forall_forall in gamma_valid.
+  rename gamma_valid into Hval.
+  pose proof (in_indpreds_of_context gamma l l_in) as Hinl.
+  destruct Hinl as [l2 [Hinl2 Hl]]; subst.
+  specialize (Hval _ Hinl2).
+  simpl in Hval.
+  destruct Hval as [_ [_ [_ Hunif]]].
+  unfold indpreds_uniform in Hunif.
+  unfold indpred_uniform in Hunif.
+  destruct l2. constructor.
+  simpl in Hunif.
+  unfold is_true in Hunif.
+  rewrite forallb_forall in Hunif.
+  rewrite Forall_concat.
+  rewrite Forall_forall. intros.
+  rewrite Forall_forall. intros. simpl.
+  destruct i; simpl in *.
+  assert (Hmapeq1: forall (l: list indpred_def),
+    map fst (get_indpred l) =
+    predsyms_of_indprop l).
+  {
+    clear. induction l; simpl; auto; destruct a; rewrite IHl; auto.
+  }
+  rewrite Hmapeq1.
+  assert (Hparamseq: (s_params p0) = s_params p). {
+    rewrite Forall_eq_iff in Halleq.
+    apply Halleq. simpl. auto.
+    apply in_bool_In in p_in; auto.
+  }
+  assert (Hmapeq2: forall (l: list indpred_def),
+    map snd (get_indpred l) =
+    map indpred_def_constrs l).
+  {
+    clear. induction l; simpl; intros; auto.
+    rewrite IHl. f_equal. destruct a; reflexivity.
+  }
+  rewrite <- Hparamseq. apply Hunif.
+  rewrite in_app_iff; destruct H; subst; auto.
+  right. rewrite in_concat. exists x. split; auto.
+  rewrite <- Hmapeq2; auto.
+Qed.
+
+Lemma indprop_fmla_valid
+  {l: list (predsym * list formula)}
+  (l_in: In l (indpreds_of_context gamma))
+  {p: predsym} {fs: list formula}
+  (p_in: In (p, fs) l)
+  {f: formula}
+  (f_in: In f fs):
+  formula_typed gamma f.
+Proof.
+  pose proof (in_indpred_valid l_in).
+  rewrite Forall_forall in H.
+  assert (In fs (map snd l)). rewrite in_map_iff.
+  exists (p, fs); auto.
+  specialize (H _ H0).
+  rewrite Forall_forall in H.
+  apply H; auto.
+Qed.
+
+End Lemmas.
+
+(*We also need [interp_with_Ps] in multiple places*)
+
+
+(*We need the following utility:*)
+Section FindApplyPred.
+
+Section Def.
+
+Context {gamma: context} 
+  (gamma_valid: valid_context  gamma) (pd: pi_dom).
+
+(*For the list of predsyms, we need to search through the list
+  to apply the correct pred. The dependent types make this
+  complicated, so we use a separate function*)
+Fixpoint find_apply_pred (pi: pi_funpred gamma_valid pd)
+(ps: list predsym)
+(*Our props are an hlist, where we have a Pi for each pi
+of type (srts -> arg_list pi srts -> bool)*)
+(Ps: hlist (fun (p: predsym) => forall srts, 
+  arg_list (domain (dom_aux pd)) 
+  (sym_sigma_args p srts) -> bool) ps) (p: predsym) :
+  (forall srts : list sort,
+    arg_list (domain (dom_aux pd)) 
+      (sym_sigma_args p srts) -> bool) :=
+  (match ps as ps' return
+  (hlist (fun p : predsym =>
+    forall srts : list sort,
+    arg_list (domain (dom_aux pd))
+      (sym_sigma_args p srts) -> bool) ps') ->
+    forall srts : list sort,
+      arg_list (domain (dom_aux pd)) 
+        (sym_sigma_args p srts) -> bool with
+  (*Underneath the depednent types, this is quite
+    simple: iterate through the list, compare for equality
+    and if so, apply the correct Pi function*)
+  | nil => fun _ => (preds gamma_valid pd pi p)
+  | p' :: ptl =>  fun Hp =>
+    match (predsym_eq_dec p p') with
+    | left Heq => ltac:(rewrite Heq; exact (hlist_hd Hp))
+    | right _ => (find_apply_pred pi ptl (hlist_tl Hp) p)
+    end
+  end) Ps.
+
+Lemma find_apply_pred_in (pf: pi_funpred gamma_valid pd)
+  (ps: list predsym)
+  (Ps: hlist
+  (fun p' : predsym =>
+    forall srts : list sort,
+    arg_list (domain (dom_aux pd)) (sym_sigma_args p' srts) -> bool)
+  ps)
+  (p: predsym)
+  (Hinp: in_bool predsym_eq_dec p ps) :
+  find_apply_pred pf ps Ps p =
+  get_hlist_elt predsym_eq_dec Ps p Hinp.
+Proof.
+  induction ps; simpl.
+  - inversion Hinp.
+  - revert Hinp. simpl. 
+    destruct (predsym_eq_dec p a); subst; auto.
+Qed.
+
+Lemma find_apply_pred_notin (pf: pi_funpred gamma_valid pd)
+(ps: list predsym)
+(Ps: hlist
+(fun p' : predsym =>
+  forall srts : list sort,
+  arg_list (domain (dom_aux pd)) (sym_sigma_args p' srts) -> bool)
+ps)
+(p: predsym) :
+~ In p ps ->
+find_apply_pred pf ps Ps p = preds gamma_valid pd pf p.
+Proof.
+  induction ps; simpl; auto.
+  intros Hnot. destruct (predsym_eq_dec p a); subst; auto.
+  exfalso. apply Hnot; auto.
+Qed.
+
+End Def.
+
+(*And we will need the following extensionality lemma
+  (for our proof system)*)
+Lemma find_apply_pred_ext {gamma1 gamma2: context}
+  (gamma_valid1: valid_context gamma1)
+  (gamma_valid2: valid_context gamma2)
+  (pd: pi_dom) 
+  (pf1 : pi_funpred gamma_valid1 pd)
+  (pf2 : pi_funpred gamma_valid2 pd)
+  (Hext: forall p srts a,
+    preds gamma_valid1 pd pf1 p srts a =
+    preds gamma_valid2 pd pf2 p srts a)
+  l Ps p srts a:
+  find_apply_pred gamma_valid1 pd pf1 l Ps p srts a =
+  find_apply_pred gamma_valid2 pd pf2 l Ps p srts a.
+Proof.
+  induction l; simpl; auto.
+  destruct (predsym_eq_dec p a0); subst; auto.
+Qed.
+
+End FindApplyPred.
+
+Section InterpPs.
+
+Context {gamma: context} 
+  (gamma_valid: valid_context  gamma) (pd: pi_dom).
+
+Section Def.
+
+(*First, define interpretations*)
+
+(*An interpretation where we substitute p with P*)
+
+Definition interp_with_P (pi: pi_funpred gamma_valid pd) (p: predsym) 
+  (P: forall srts, 
+    arg_list (domain (dom_aux pd)) (sym_sigma_args p srts) -> bool) :
+  pi_funpred gamma_valid pd :=
+  {|
+    funs := funs gamma_valid pd pi;
+    preds := (fun pr : predsym =>
+    match predsym_eq_dec p pr with
+    | left Heq =>
+        match Heq with
+        | eq_refl => P
+        end
+    | _ => preds gamma_valid pd pi pr
+    end);
+    adt_props := adt_props gamma_valid pd pi
+  |}.
+
+Notation find_apply_pred := (find_apply_pred gamma_valid pd).
+
+(*Do the same for a list of predsyms*)
+Definition interp_with_Ps (pi: pi_funpred gamma_valid pd)
+  (ps: list predsym)
+  (*Our props are an hlist, where we have a Pi for each pi
+  of type (srts -> arg_list pi srts -> bool)*)
+  (Ps: hlist (fun (p: predsym) => forall srts, 
+    arg_list (domain (dom_aux pd)) 
+    (sym_sigma_args p srts) -> bool) ps) :
+  pi_funpred gamma_valid pd :=
+  {|
+  funs := funs gamma_valid pd pi;
+  preds := find_apply_pred pi ps Ps;
+  adt_props := adt_props gamma_valid pd pi
+|}.
+
+Lemma interp_with_Ps_single (pi: pi_funpred gamma_valid pd)
+  (p: predsym)
+  (Ps: hlist (fun (p:predsym) => forall srts, 
+    arg_list (domain (dom_aux pd)) 
+    (sym_sigma_args p srts) -> bool) [p]) :
+  interp_with_Ps pi [p] Ps =
+  interp_with_P pi p (hlist_hd Ps).
+Proof.
+  unfold interp_with_Ps. simpl.
+  unfold interp_with_P. f_equal.
+  apply functional_extensionality_dep. intros p'.
+  destruct (predsym_eq_dec p' p).
+  - subst. destruct (predsym_eq_dec p p); simpl; [|contradiction].
+    assert (e = eq_refl) by (apply UIP_dec; apply predsym_eq_dec).
+    rewrite H. reflexivity.
+  - destruct (predsym_eq_dec p p'); subst; auto.
+    contradiction.
+Qed.
+
+End Def.
+End InterpPs.
