proofs/core/Interp2.v
@@ -1,0 +1,23 @@
+(*Contains the definition of [pi_dom_full], formerly part of the
+  definition of [pi_dom] in Interp.v but now describing a particular
+  interpretation that happens to set all ADT interps to W-types.
+  We show in ADTFullProps.v that [pi_dom_full] satisfies
+  the ADT spec in [pi_funpred] and in ADTInterp.v give the explicit
+  construction of such an interp.*)
+Require Export Interp IndTypes.
+
+
+Record pi_dom_full (gamma: context) (pd: pi_dom) := {
+  
+
+  (*ADTs: they are the corresponding W type created by [mk_adts],
+    with the typesym and typevar map coming from sorts on which
+    the type is applied*)
+
+    adts: forall (m: mut_adt) (srts: list sort)
+    (a: alg_datatype) (m_in: mut_in_ctx m gamma) (Hin: adt_in_mut a m)
+    (Hlen: length srts = length (m_params m)),
+    (domain (dom_aux pd)) (s_cons (adt_name a) srts) =
+    IndTypes.adt_rep m srts (dom_aux pd) a Hin;
+
+}.
